still need to update controller

examples/airlock.v
@@ -11,12 +11,15 @@ From mathcomp Require Import all_boot classical_sets.
 From FreerDPS Require Import Core Freer Hoare HoareFacts.
 From examples Require Import airlock_helper.
 
-Import SpecializedHoareModule.
+Import SpecializedHoareModule FreerFuns.
+Generalizable All Variables.
 
-Create HintDb airlock.
 
 (** * Specifying *)
+(* Opaque denote. *)
 
+
+Module Export DoorsControllerM.
 (** ** Doors *)
 
 Inductive door : Type := left | right.
@@ -27,42 +30,27 @@ Inductive DOORS : effect :=
 | IsOpen : door -> DOORS bool
 | Toggle : door -> DOORS unit.
 
-Generalizable All Variables.
+Section doors_s.
+Context `{Provide Fx DOORS} {im : freerMonad Fx}.
 
-Section airlock_s.
-
-Import FreerFuns.
-
-Definition is_open `{Provide Fx DOORS} {im : freerMonad Fx} (d : door) :
-    im bool :=
-  trigger (inj_p $ IsOpen d).
-
-Definition toggle `{Provide Fx DOORS} {im : freerMonad Fx} (d : door) :
-    im unit :=
-  trigger (inj_p $ Toggle d).
-
-Definition open_door `{Provide Fx DOORS} {im : freerMonad Fx}
-    (d : door) : im unit :=
-  is_open d >>= fun open =>
-  when (~~ open) (toggle d).
-
-Definition close_door `{Provide Fx DOORS} {im : freerMonad Fx}
-    (d : door) : im unit :=
-  is_open d >>= fun open =>
-  when open (toggle d).
-
+Definition is_open (d : door) : im bool := trigger $ IsOpen d.
+Definition toggle (d : door) : im unit := trigger $ Toggle d.
+Definition open_door (d : door) : im unit :=
+  is_open d >>= fun open => when (~~ open) (toggle d).
+Definition close_door (d : door) : im unit :=
+  is_open d >>= (when ^~ (toggle d)).
+End doors_s.
 (** ** Controller *)
 
 Inductive CONTROLLER : effect :=
 | Tick : CONTROLLER unit
 | RequestOpen (d : door) : CONTROLLER unit.
 
-Definition tick `{Provide Fx CONTROLLER} {im : freerMonad Fx} : im unit :=
-  trigger (inj_p Tick).
-
-Definition request_open `{Provide Fx CONTROLLER} {im : freerMonad Fx}
-    (d : door) : im unit :=
-  trigger (inj_p $ RequestOpen d).
+Section controller_s.
+Context `{Provide Fx CONTROLLER} {im : freerMonad Fx}.
+Definition tick : im unit := trigger Tick.
+Definition request_open (d : door) : im unit := trigger $ RequestOpen d.
+End controller_s.
 
 Definition co (d : door) : door :=
   match d with
@@ -74,25 +62,7 @@ Lemma co_leftE : co left = right.
 Proof. by []. Qed.
 
 Definition controller `{Provide Fx DOORS, Provide Fx (STORE nat)}
-    {im : freerMonad Fx} : component (im:=im) CONTROLLER Fx
-  (* .
-  move=> X; case=> [|d].
-  - apply/bind=>[|cpt].
-    + apply/iget.
-    + apply/when.
-      * apply: (15 <? cpt).
-      * apply/bind=>[|_].
-      -- apply/close_door/left.
-      -- apply/bind=>[|_].
-        ++ apply/close_door/right.
-        ++ apply/iput/0.
-  - apply/bind=>[|_].
-    + apply/close_door/co/d.
-    + apply/bind=>[|_].
-      * apply/open_door/d.
-      * apply/iput/0.
-  Show Proof. *)
-   :=
+    {im : freerMonad Fx} : component (im:=im) CONTROLLER Fx :=
   fun _ op =>
     match op with
     | Tick =>
@@ -106,12 +76,13 @@ Definition controller `{Provide Fx DOORS, Provide Fx (STORE nat)}
       open_door d >>
       iput 0%nat
     end.
+End DoorsControllerM.
 
 (** * Verifying the Airlock Controller *)
 
 (** ** Doors Specification *)
 
-(** *** Witness States *)
+(* ----------------------------- Witness States ----------------------------- *)
 
 Definition Ω : Type := bool * bool.
 (*         S : Type := left * rght. *)
@@ -136,6 +107,10 @@ Lemma tog_equ_2 (d : door) (ω : Ω)
   : sel (co d) (tog d ω) = sel (co d) ω.
 Proof. by case: d. Qed.
 
+Opaque tog.
+
+(* -------------------------------------------------------------------------- *)
+
 (** From now on, we will reason about [tog] using [tog_equ_1] and [tog_equ_2].
     FreeSpec tactics rely heavily on [cbn] to simplify certain terms, so we use
     the <<simpl never>> options of the [Arguments] vernacular command to prevent
@@ -145,9 +120,7 @@ Proof. by case: d. Qed.
     trick to prevent [cbn] to unfold impure computations covered by intermediary
     theorems. *)
 
-#[local] Opaque tog.
-Opaque denote.
-
+(* -------------------------------- Contract -------------------------------- *)
 (* Ω = bool * bool : doors state *)
 Definition step (ω : Ω) (a : Type) (op : DOORS a) (_ : a) : Ω :=
   if op is Toggle d then tog d ω else ω.
@@ -162,7 +135,6 @@ Inductive doors_o_caller : Ω -> forall (a : Type), DOORS a -> Prop :=
       [co d] has to be closed too for a request to toggle [d] to be valid. *)
 | req_toggle (d : door) (ω : Ω) (H : sel (co d) ω -> sel d ω)
   : doors_o_caller ω unit (Toggle d).
-  (* H : ~~ sel (co d) ω *)
 
 (** *** Promises / PostCondition *)
 Inductive doors_o_callee : Ω -> forall (a : Type), DOORS a -> a -> Prop :=
@@ -175,34 +147,25 @@ Inductive doors_o_callee : Ω -> forall (a : Type), DOORS a -> a -> Prop :=
 | doors_o_callee_toggle (d : door) (ω : Ω) (x : unit)
   : doors_o_callee ω unit (Toggle d) x.
 
-Definition doors_contract : contract DOORS Ω :=
+(* doors_c => {{door_caller}} p%step {{door_callee}} *)
+Definition doors_c : contract DOORS Ω :=
   make_contract step doors_o_caller doors_o_callee.
-(* => {{door_caller}} p%step {{door_callee}} *)
+(* -------------------------------------------------------------------------- *)
 
-Lemma doors_effect_preE {Fx a} `{MayProvide Fx DOORS}
-    (op : Fx a) (ω : Ω) :
-  pre (hoare_of_contract doors_contract op) ω <->
+Section doors_pre_post_helpers.
+Context `{Provide Fx DOORS} {a : Type}.
+
+Lemma doors_effect_preE (op : Fx a) (ω : Ω) :
+  pre (hoare_of_contract doors_c op) ω <->
   match proj_p op with
   | Some door_op => doors_o_caller ω a door_op
   | None => True
   end.
 Proof. by rewrite /hoare_of_contract /= /gen_caller_obligation. Qed.
 
-Lemma doors_o_caller_preE `{Provide Fx DOORS} {a}
-    (ω : Ω) (op : DOORS a) :
-  pre (hoare_of_contract doors_contract (inj_p op)) ω <->
-  doors_o_caller ω a op.
-Proof. by rewrite doors_effect_preE proj_inj_p_equ. Qed.
-
-Lemma doors_o_caller_preI `{Provide Fx DOORS} {a}
-    (ω : Ω) (op : DOORS a) :
-  doors_o_caller ω a op ->
-  pre (hoare_of_contract doors_contract (inj_p op)) ω.
-Proof. by rewrite doors_o_caller_preE. Qed.
-
-Lemma doors_effect_postE {Fx a} `{MayProvide Fx DOORS}
+Lemma doors_effect_postE
     (op : Fx a) (ω : Ω) (x : a) (ω' : Ω) :
-  post (hoare_of_contract doors_contract op) ω x ω' <->
+  post (hoare_of_contract doors_c op) ω x ω' <->
   match proj_p op with
   | Some door_op =>
       ω' = step ω a door_op x /\ doors_o_callee ω a door_op x
@@ -216,132 +179,72 @@ case: (proj_p op)=> [door_op |] /=.
 by split=> [[-> _] | ->].
 Qed.
 
-Lemma doors_o_callee_postE `{Provide Fx DOORS} {a}
+Lemma doors_pre_condE
+    (ω : Ω) (op : DOORS a) :
+  pre (hoare_of_contract doors_c (inj_p op)) ω <->
+  doors_o_caller ω a op.
+Proof. by rewrite doors_effect_preE proj_inj_p_equ. Qed.
+
+Lemma doors_post_condE
     (ω : Ω) (op : DOORS a) (x : a) (ω' : Ω) :
-  post (hoare_of_contract doors_contract (inj_p op)) ω x ω' <->
+  post (hoare_of_contract doors_c (inj_p op)) ω x ω' <->
   ω' = step ω a op x /\ doors_o_callee ω a op x.
 Proof. by rewrite doors_effect_postE proj_inj_p_equ. Qed.
-
-Lemma doors_other_effect_postE {Fx a} `{MayProvide Fx DOORS}
-    (op : Fx a) (other : proj_p op = None)
-    (ω : Ω) (x : a) (ω' : Ω) :
-  post (hoare_of_contract doors_contract op) ω x ω' <-> ω' = ω.
-Proof.
-by rewrite doors_effect_postE other.
-Qed.
+End doors_pre_post_helpers.
 
 Opaque hoare_of_contract.
 
-(** ** Intermediary Lemmas *)
-Lemma doors_is_open_calleeE (ω : Ω) (d : door) (x : bool) :
-  doors_o_callee ω bool (IsOpen d) x -> sel d ω = x.
-Proof. by case: x=> postc; inversion postc; ssubst. Qed.
+(*--------------------------- Intermediary Lemmas ----------------------------*)
+Section IntermLemmaS.
+Context `{Provide Fx DOORS} (ω : Ω) (d : door).
 
-Lemma doors_is_open_effect_retE `{Provide Fx DOORS}
-    (ω : Ω) (d : door) (opened : bool) (ω' : Ω) :
-  post (hoare_of_contract doors_contract
+Lemma doors_is_open_post_retE (opened : bool) (ω' : Ω) :
+  post (hoare_of_contract doors_c
           (A := bool) (inj_p (IsOpen d))) ω opened ω' <->
   post (@ret (hoare Ω) bool (sel d ω)) ω opened ω'.
 Proof.
-rewrite doors_o_callee_postE hoare_pure_postE /=.
-split=> [ [-> callee] | [<- <-] ]; split=> //.
-- exact: doors_is_open_calleeE callee.
+rewrite doors_post_condE hoare_pure_postE;
+  split=> [ [-> callee] | [<- <-] ];
+  split=> //.
+- by inversion callee; ssubst.
 - exact: doors_o_callee_is_open.
 Qed.
 
-Lemma doors_is_open_effect_ret_callerE `{Provide Fx DOORS}
-    (ω : Ω) (d : door) :
-  pre (hoare_of_contract doors_contract
+Lemma doors_is_open_preE :
+  pre (hoare_of_contract doors_c
           (A := bool) (inj_p (IsOpen d))) ω <->
   pre (@ret (hoare Ω) bool (sel d ω)) ω.
 Proof.
 by rewrite hoare_pure_preE; split=> // _;
-  apply: doors_o_caller_preI; exact: req_is_open.
+  rewrite doors_pre_condE;
+  exact: req_is_open.
 Qed.
 
-Lemma doors_toggle_effect_postE `{Provide Fx DOORS}
-  (ω : Ω) (d : door) (u : unit) (ω' : Ω) :
-  post (hoare_of_contract doors_contract
+Lemma doors_toggle_postE (u : unit) (ω' : Ω) :
+  post (hoare_of_contract doors_c
           (A := unit) (inj_p (Toggle d))) ω u ω' <->
   ω' = tog d ω.
 Proof.
-by rewrite doors_o_callee_postE;
+by rewrite doors_post_condE;
   split=> [ [-> _] | ->] //; split=>//;
   exact: doors_o_callee_toggle.
 Qed.
 
-Lemma doors_toggle_effect_ret_callerE `{Provide Fx DOORS}
-    (ω : Ω) (d : door)
+Lemma doors_toggle_preE
     (* Safe : porte 1 ferméE -> porte 2 ferméE *)
     (* (safe : sel d ω = false -> sel (co d) ω = false) *)
     (safe : sel (co d) ω -> sel d ω) :
-  pre (hoare_of_contract doors_contract
+  pre (hoare_of_contract doors_c
           (A := unit) (inj_p (Toggle d))) ω <->
   pre (@ret (hoare Ω) unit tt) ω.
 Proof.
 by rewrite hoare_pure_preE; split=> // _;
-  apply: doors_o_caller_preI; exact: req_toggle safe.
+  rewrite doors_pre_condE;
+  exact: req_toggle safe.
 Qed.
+End IntermLemmaS.
 
-
-Lemma doors_toggle_callerE (ω : Ω) (d : door) :
-  doors_o_caller ω unit (Toggle d) ->
-  sel (co d) ω -> sel d ω.
-Proof. by move: ω d=> [[|] [|]] [|] //=; inversion 1. Qed.
-
-(** Closing a door [d] in any system [ω] is always a respectful operation. *)
 Local Open Scope classical_set_scope.
-
-
-(* TODO(cleanup): Check whether this proof can be shortened. *)
-Lemma close_door_respectful `{Provide Fx DOORS} {im : freerMonad Fx}
-    (d : door) :
-  pre (to_hoare (im:=im) doors_contract (close_door d)) = [set: _].
-Proof.
-rewrite /close_door -subTset=> ω _; apply: to_hoare_bind_preI.
-- by rewrite to_hoare_requestE doors_is_open_effect_ret_callerE.
-move=> [|] ω';
-  rewrite to_hoare_when_preE // to_hoare_requestE doors_is_open_effect_retE
-  => -[d_open <-].
-by rewrite to_hoare_requestE;
-  apply/(doors_toggle_effect_ret_callerE ω d).
-Qed.
-
-(* TODO(cleanup): Check whether this proof can be shortened. *)
-Lemma open_door_respectful `{Provide Fx DOORS} {im : freerMonad Fx}
-    (ω : Ω) (d : door) (safe : ~~ sel (co d) ω) :
-  pre (to_hoare (im:=im) doors_contract
-    (open_door (Fx := Fx) d)) ω.
-Proof.
-rewrite /open_door; apply: to_hoare_bind_preI.
-- by rewrite to_hoare_requestE doors_is_open_effect_ret_callerE.
-move=> [|] ω'; rewrite to_hoare_when_preE //
-  to_hoare_requestE doors_is_open_effect_retE
-  => -[_ <-].
-rewrite to_hoare_requestE;
-  apply/(doors_toggle_effect_ret_callerE ω d)=>//.
-by move: safe=> /[swap] ->.
-Qed.
-
-Lemma close_door_run `{Provide Fx DOORS} {im : freerMonad Fx}
-  (ω : Ω) (d : door) (ω' : Ω) (x : unit)
-  (run : post (to_hoare (im:=im) doors_contract (close_door d)) ω x ω') :
-~~ sel d ω'.
-Proof.
-move: run; rewrite /close_door to_hoare_bind_postE.
-move=> [opened [? [ ]]].
-rewrite to_hoare_requestE doors_is_open_effect_retE to_hoare_when_postE
-  => -[+ <-].
-case: opened.
-- by move=> + [[] ];
-  rewrite to_hoare_requestE doors_toggle_effect_postE=> /[swap] ->;
-  rewrite tog_equ_1=> ->.
-by move=> /[swap] -> ->.
-Qed.
-
-#[local] Opaque close_door.
-#[local] Opaque open_door.
-#[local] Opaque Nat.ltb.
 
 Remark one_door_safe_all_doors_safe (ω : Ω) (d : door)
     (safe : ~~sel d ω \/ ~~sel (co d) ω)
@@ -350,20 +253,66 @@ Proof.
 by move: d safe=> + /[swap]; case; case=>//=; rewrite or_comm.
 Qed.
 
+Definition doors_safe (ω : Ω) := ~~ sel left ω \/ ~~ sel right ω.
+
+Section RespectfulAndRunLemmas.
+Context `{Provide Fx DOORS} {im : freerMonad Fx}.
+(** Closing a door [d] in any system [ω] is always a respectful operation. *)
+Lemma close_door_respectful (d : door) :
+  pre (to_hoare (im:=im) doors_c (close_door d)) = [set: _].
+Proof.
+rewrite /close_door -subTset=> ω _; apply: to_hoare_bind_preI.
+- by rewrite to_hoare_requestE doors_is_open_preE.
+move=> [|] ?;
+  rewrite to_hoare_when_preE // to_hoare_requestE doors_is_open_post_retE
+  => -[? <-].
+by rewrite to_hoare_requestE;
+  apply/(doors_toggle_preE ω d).
+Qed.
+
+Lemma open_door_respectful (ω : Ω) (d : door) (safe : ~~ sel (co d) ω) :
+  pre (to_hoare (im:=im) doors_c
+    (open_door (Fx := Fx) d)) ω.
+Proof.
+rewrite /open_door; apply: to_hoare_bind_preI.
+- by rewrite to_hoare_requestE doors_is_open_preE.
+move=> [|] ?;
+  rewrite to_hoare_when_preE // to_hoare_requestE doors_is_open_post_retE
+  => -[_ <-].
+rewrite to_hoare_requestE;
+  apply/(doors_toggle_preE ω d)=>//.
+by move: safe=> /[swap] ->.
+Qed.
+
+Lemma close_door_run (ω : Ω) (d : door) (ω' : Ω) (x : unit)
+  (run : post (to_hoare (im:=im) doors_c (close_door d)) ω x ω') :
+~~ sel d ω'.
+Proof.
+move: run; rewrite /close_door to_hoare_bind_postE.
+move=> [opened [? [ ]]].
+rewrite to_hoare_requestE doors_is_open_post_retE to_hoare_when_postE
+  => -[+ <-].
+case: opened; last first.
+- by move=> /[swap] -> ->.
+by move=> + [[] ];
+  rewrite to_hoare_requestE doors_toggle_postE=> /[swap] ->;
+  rewrite tog_equ_1=> ->.
+Qed.
+
+Opaque close_door.
+Opaque open_door.
+Opaque Nat.ltb.
+
 (** The objective of this lemma is to prove that, if either the right door or
     the left door is closed, then after any respectful run of a computation
     [p] that interacts with doors, this fact remains true. *)
 
-#[local] Opaque sel.
-Definition doors_safe (ω : Ω) :=
-  ~~ sel left ω \/ ~~ sel right ω.
+Opaque sel.
 
-(* TODO(cleanup): Check whether this proof can be shortened. *)
-Lemma doors_request_preserves_safe `{Provide Fx DOORS}
-    {im : freerMonad Fx}
+Lemma doors_request_preserves_safe
     `(op : Fx a) (ω : Ω) (x : a) (ω' : Ω) :
-  pre (to_hoare (im:=im) doors_contract (trigger op)) ω ->
-  post (to_hoare (im:=im) doors_contract (trigger op)) ω x ω' ->
+  pre (to_hoare (im:=im) doors_c (trigger op)) ω ->
+  post (to_hoare (im:=im) doors_c (trigger op)) ω x ω' ->
   doors_safe ω -> doors_safe ω'.
 Proof.
 rewrite to_hoare_requestE doors_effect_preE doors_effect_postE.
@@ -379,82 +328,54 @@ by inversion caller as [|?? Hsafe]; subst;
   move: co_open Hsafe d_closed=> -> ->.
 Qed.
 
-Lemma doors_handler_preserves_safe `{Provide Fx DOORS}
-    {im : freerMonad Fx} {A} (op : Fx A) :
-  preserves_invariant doors_safe
-    (hoare_of_contract doors_contract op).
+Lemma doors_handler_preserves_safe `(op : Fx a) :
+  preserves_invariant doors_safe (hoare_of_contract doors_c op).
 Proof.
 by move=> state result state' op_pre op_post state_safe;
-  apply: (doors_request_preserves_safe (im:=im) op state result state');
+  apply: (doors_request_preserves_safe op state result state');
   rewrite ?to_hoare_requestE.
 Qed.
 
-Lemma doors_run_preserves_safe `{Provide Fx DOORS}
-    {A} (p : freer Fx A) :
-  preserves_invariant doors_safe
-    (p |= doors_contract).
+(** /!\ WARNING: This proof exits the Equational Reasoning.
+  * This is a known issue. I need to find a way to remove this
+  * induction but can't find one right now.
+  *)
+Lemma doors_run_preserves_safe `(p : freer Fx A) :
+  preserves_invariant doors_safe (p |= doors_c).
 Proof.
 elim: p=> [value | X op k IH].
 - by rewrite to_hoare_localE; exact: preserves_invariant_ret.
-exact: (preserves_invariant_bind
-  (doors_handler_preserves_safe (im:=freer Fx) op) IH).
+exact: (preserves_invariant_bind (doors_handler_preserves_safe op) IH).
 Qed.
 
-Lemma respectful_run_inv `{Provide Fx DOORS} {A} (p : freer Fx A)
+Lemma respectful_run_inv `(p : im A)
     (ω : Ω) (safe : ~~ sel left ω \/ ~~ sel right ω)
     (a : A) (ω' : Ω)
-    (hpre : pre (to_hoare (im:=freer Fx) doors_contract p) ω)
-    (hpost : post (to_hoare (im:=freer Fx) doors_contract p) ω a ω') :
+    (hpre : pre (p |= doors_c) ω)
+    (hpost : post (p |= doors_c) ω a ω') :
   ~~ sel left ω' \/ ~~ sel right ω'.
-(** The induction in [doors_run_preserves_safe] reduces this proof to showing
-    that every handled request preserves [doors_safe]. It accounts for the
-    following two cases:
-
-    - Either [p] is a pure computation; in such a case, the doors state
-      does not change, hence the proof is trivial.
-
-    - Or [p] consists in a request to the doors effect, and a continuation
-      whose domain satisfies the theorem, i.e. it preserves the invariant that
-      either the left or the right door is closed.  Due to this hypothesis, we
-      only have to prove that the first request made by [p] does not break the
-      invariant. We consider two cases.
-
-      - Either the computation asks for the state of a given door ([IsOpen]),
-        then again the doors state does not change and the proof is trivial.
-      - Or the computation wants to toggle a door [d].  We know by hypothesis
-        that either [d] is closed or [d] is open (thanks to the
-        [one_door_safe_all_doors_safe] result and the [safe] hypothesis).
-        Again, we consider both cases.
-
-         - If [d] is closed —and therefore will be opened—, then because we
-           consider a respectful run, [co d] is necessarily closed too (it is a
-           requirements of [door_contract]). Once [d] is opened, [co d] is still
-           closed.
-         - Otherwise, [co d] is closed, which means once [d] is toggled (no
-           matter its initial state), then [co d] is still closed.
-
-         That is, we prove that, when [p] toggles [d], [co d] is necessarily
-         closed after the request has been handled.  Because there is at least
-         one door closed ([co d]), we can conclude that either the right or the
-         left door is closed thanks to [one_door_safe_all_doors_safe]. *)
 Proof.
-by move: hpre hpost safe; exact: doors_run_preserves_safe.
+by move: hpre hpost safe;
+  rewrite -to_hoare_reifyE;
+  exact: doors_run_preserves_safe.
 Qed.
+End RespectfulAndRunLemmas.
 
 (** ** Main Theorem *)
 (* TODO(cleanup): Check whether this proof can be shortened. *)
+
+Section theo_cont.
 Theorem controller_correct
-    `{StrictProvide2 Fx DOORS (STORE nat)}
+    `{StrictProvide2 Fx DOORS (STORE nat)} {im : freerMonad Fx}
   : correct_component controller
-    (im:=freer Fx)
+    (im:=im)
     (no_contract CONTROLLER)
-    doors_contract
+    doors_c
     (fun _ ω => ~~ sel left ω \/ ~~ sel right ω).
 Proof.
 rewrite /correct_component=> ωF ω safe α op _.
 have controller_pre :
-    pre (to_hoare doors_contract
-      (controller (im:=freer Fx) α op)) ω.
+    pre ((controller (im:=im) α op) |= doors_c) ω.
   case: op=> [|d]; rewrite /controller.
   - apply: to_hoare_bind_preI.
     + exact: to_hoare_distinguished_request_preI.
@@ -470,13 +391,11 @@ have controller_pre :
   - apply: to_hoare_bind_preI.
     + by rewrite close_door_respectful.
     move=> result state close_post.
-    exact: (open_door_respectful (Fx:=Fx) (im:=freer Fx) state d
+    exact: (open_door_respectful (Fx:=Fx) (im:=im) state d
       (close_door_run ω (co d) state result close_post)).
   by move=> result state body_post;
     exact: to_hoare_distinguished_request_preI.
 split=> // x ω' run; split; first exact: mk_no_callee_obligation.
-exact: (respectful_run_inv (Fx:=Fx)
-  (controller (im:=freer Fx) α op) ω safe x ω' controller_pre run).
+exact: (respectful_run_inv (Fx:=Fx) (im:=im)
+  (controller (im:=im) α op) ω safe x ω' controller_pre run).
 Qed.
-
-End airlock_s.
